Proofs for translation of types (and boxed translation). Some progress on the case for Pi-types

forcing/Soundness.v
@@ -22,7 +22,11 @@ Definition ft_term c Σ σ :=
   (snd (otranslate (Environ.of_global_context Σ) (mkFCtxt σ cat []) tt c)).
 
 Definition ft_ctx Γ Σ σ  :=
-  (snd (otranslate_context (Environ.of_global_context Σ) (mkFCtxt σ cat []) tt Γ)).
+  (otranslate_context_no_sigma (Environ.of_global_context Σ) (mkFCtxt σ cat []) tt Γ).
+
+Definition ft_type_boxed c Σ σ  :=
+  (snd (otranslate_boxed_type otranslate (Environ.of_global_context Σ) (mkFCtxt σ cat []) tt c)).
+
 
 Definition leq_refl sigma t : leq_term sigma t t = true.
   induction t.
@@ -56,11 +60,26 @@ Proof.
       (* NOTE: something is not right, either [wf_graph] or [init_graph] *)
 Admitted.
 
+Lemma typed_empty_global_env :
+  type_global_env init_graph [].
+Proof.
+  constructor. apply wf_init_graph.
+Qed.
 
 Ltac setctx na :=
   match goal with
-    |- ?Σ ;;; ?Γ |- _ : _ => set(na := Γ)
+    [ |- ?Σ ;;; ?Γ |- _ : _ ] => set(na := Γ)
+  | [|- type_local_env ?Σ ?Γ ] => set(na := Γ)
   end.
+
+Ltac setctx_2 na :=
+  match goal with
+    |- ?Σ ;;; ?Γ ,, ?v2 ,, ?v1 |- _ : _ => set(na := [v1;v2])
+  | |- type_local_env ?Σ ?Γ => match Γ with
+                               | ?v1 :: ?v2 :: _ => set(na := [v1;v2])
+                               end
+  end.
+
 
 Ltac solve_rel :=
   let Γ' := fresh "Γ" in
@@ -77,7 +96,7 @@ Reserved Notation "E ## Γ |= σ" (at level 40).
 (* TODO: think about the empty context case *)
 Inductive fctx_valid E : context -> list forcing_condition -> Type :=
 | fctx_valid_nil : E ## vass (nNamed "p") Relevant (tConst "Obj" nil) :: nil |= nil
-| fctx_valid_cons_var Γ σ T t : E ## Γ |= σ -> (to_global_context E) ;;; Γ |- t : T ->
+| fctx_valid_cons_var Γ σ T : E ## Γ |= σ ->
                             E ## (Γ ,, vass (nNamed "t") Relevant T) |= (σ ,, fcVar)
 | fctx_valid_cons_lift Γ σ : E ## Γ |= σ ->
                         E ## (Γ ,,, get_ctx_lift cat E (last_condition σ)) |= (σ ,, fcLift)
@@ -89,8 +108,8 @@ Lemma last_condition_sound σ Γ (Σ := ([], init_graph)) :
   (of_global_context Σ) ## Γ |= σ ->
   Σ ;;; Γ |- tRel (last_condition σ) : cat_obj.
 Proof.
-  intros TyCtx FCvalid.
-  induction FCvalid.
+  intros TyCtx FcValid.
+  induction FcValid.
   - simpl. solve_rel.
   - simpl.
     pose [vass (nNamed "t") Relevant T] as Γ'.
@@ -98,41 +117,47 @@ Proof.
     assert (TyCtxΓ : type_local_env Σ Γ).
     { inversion TyCtx;subst;auto. }
     apply weakening.
-    + simpl. constructor. apply wf_init_graph.
+    + apply typed_empty_global_env.
     + simpl.
       (* NOTE: here we do inversion again, because of some issues with [typing] being in [Type] *)
       inversion TyCtx;subst;auto.
-    + apply IHFCvalid; eauto.
+    + apply IHFcValid; eauto.
   - solve_rel.
 Qed.
 
+Lemma lift_sound (Σ := (nil,init_graph)) Γ σ v :
+  type_local_env Σ Γ ->
+  (of_global_context Σ) ## Γ |= σ ->
+  Σ;;; Γ,, vass v Relevant cat_obj |- tApp cat_hom [tRel (S (last_condition σ)); tRel 0] : sort_set.
+Proof.
+  intros TyCtx FcValid.
+  eapply hom_sort.
+  - pose ([vass v Relevant cat_obj]) as Γ'.
+    change
+      (Σ;;; Γ ,,, Γ' |- lift0 #|Γ'| (tRel (last_condition σ)) : lift0 #|Γ'| cat_obj).
+    apply weakening with (Γ' := Γ').
+    * apply typed_empty_global_env.
+    * simpl. constructor. apply TyCtx. econstructor. simpl. apply obj_sort.
+    * apply last_condition_sound;eauto.
+  - solve_rel.
+Qed.
 
 Lemma lam_q_f_sound (Σ := (nil,init_graph)) Γ σ t T :
   let E := (of_global_context Σ) in
   let fctx := (mkFCtxt σ cat []) in
   let ext := get_ctx_lift cat E (last_condition σ) in
   type_local_env Σ Γ ->
+  (of_global_context Σ) ## Γ |= σ ->
   Σ ;;; Γ ,,, ext |- t : T ->
   Σ ;;; Γ |- snd (λ_q_f E fctx) t : snd (Π_q_f E fctx) T.
 Proof.
-  simpl. intros TyCtx Ty.
+  simpl. intros TyCtx FcValid Ty.
   econstructor.
   + eapply obj_sort.
   + econstructor.
-    * eapply hom_sort.
-      ** pose (vass pos_name Relevant (cat_obj) :: nil) as Γ'.
-         change
-           (Σ;;; Γ ,,, Γ' |- lift0 #|Γ'| (tRel (last_condition σ)) : lift0 #|Γ'| cat_obj).
-         apply weakening with (Γ' := Γ').
-         *** simpl. constructor. apply wf_init_graph.
-         *** simpl. constructor. apply TyCtx. econstructor. simpl. apply obj_sort.
-         *** apply last_condition_sound.
-             (* TODO : add Γ typed assumption *)
-             admit.
-             (* TODO : add forcing context validity assumption *)
-             admit.
-      ** solve_rel.
-  Admitted.
+    * apply lift_sound;eauto.
+    * eauto.
+Qed.
 
 Lemma Π_q_f_lift_sound (Σ := (nil,init_graph)) Γ σ T l :
   let σ_ext := σ ,, fcLift in
@@ -153,10 +178,10 @@ Proof.
      *** eauto.
 Qed.
 
-
-Notation "'[' c ']ᵗ' " := (ft_term c) (at level 40).
+Notation "'[' c ']ᵗ' " := (ft_term c) (at level 0).
 Notation "⟦ Γ ⟧" := (ft_ctx Γ)  (at level 40).
 Notation "'⟦' c '⟧ᵀ'" := (ft_type c) (at level 40).
+Notation "'⟦' c '⟧!'" := (ft_type_boxed c) (at level 40).
 
 Lemma context_traslation_valid E Γ σ :
   let Σ := to_global_context E in
@@ -190,41 +215,126 @@ Lemma sort_translation_prefix_sound (Σ := (nil,init_graph)) σ Γ T l:
   let ext1 := get_ctx_lift cat E (last_condition σ) in
   let ext2 := get_ctx_lift cat E (last_condition (σ ,, fcLift)) in
   type_local_env Σ Γ ->
+  (of_global_context Σ) ## Γ |= σ ->
   Σ ;;; Γ ,,, ext1 ,,, ext2  |- T : tSort l ->
   Σ ;;; Γ |- snd (sort_translation_prefix E fctx tt) T
                       : snd (Π_q_f E fctx) srt.
 Proof.
-  intros ? ? ? ? ? TyΓ TyT.
+  intros ? ? ? ? ? TyCtx FcValid TyT.
   simpl.
-  apply lam_q_f_sound;simpl.
-  - assumption.
-  - unfold sort_set.
-    eapply Π_q_f_lift_sound. apply TyT.
+  apply lam_q_f_sound;simpl;eauto.
+  unfold sort_set.
+  eapply Π_q_f_lift_sound. apply TyT.
 Qed.
 
-Lemma forcing_typing_soundness (Σ := (nil,init_graph)) Γ t T σ  :
+Lemma type_translation_sound (Σ := ([],init_graph)) Γ σ T :
+  type_local_env Σ Γ ->
+  (of_global_context Σ) ## Γ |= σ ->
+  Σ;;; Γ |- [T ]ᵗ Σ σ : (⟦ tSort [Universe.Expr.set] ⟧ᵀ) Σ σ ->
+  Σ ;;; Γ |- ⟦T⟧ᵀ Σ σ : tSort [Universe.Expr.set].
+Proof.
+  intros TyCtx FcValid TyT.
+  unfold ft_type,otranslate_type. simpl. unfold mkOptApp.
+  remember (tRel (last_condition σ)) as last_fcond.
+  remember (tApp (tConst "Id_hom" []) [last_fcond]) as id_hom_lfc.
+  change (Σ;;; Γ |- tApp ([T]ᵗ Σ σ) [last_fcond; id_hom_lfc] : tSort [Universe.Expr.set]).
+  eapply type_App.
+  - eapply TyT.
+  - unfold ft_type. simpl. unfold mkOptApp. econstructor.
+    * (* Abstract this reduction to a tactic *)
+      eapply cumul_red_r. Focus 2.
+      eapply red_beta. simpl.
+      eapply cumul_red_r. Focus 2.
+      eapply red_beta. simpl.
+      eapply cumul_refl. apply leq_refl.
+    * subst. apply last_condition_sound;eauto.
+    * econstructor. Focus 2.
+      subst. apply id_hom_type. apply last_condition_sound;eauto.
+      econstructor. subst. eapply leq_refl.
+      econstructor.
+Qed.
+
+Lemma ctx_with_lift_sound (Σ := ([],init_graph)) Γ σ:
+  let ext := get_ctx_lift cat (of_global_context Σ) (last_condition σ) in
+  type_local_env Σ Γ ->
+  (of_global_context Σ) ## Γ |= σ ->
+  type_local_env Σ (Γ ,,, ext).
+Proof.
+  simpl. intros TyCtx FcValid.
+  constructor;eauto.
+  constructor;eauto.
+  econstructor; apply obj_sort.
+  econstructor; apply lift_sound;eauto.
+Qed.
+
+Lemma boxed_type_translation_sound (Σ := ([],init_graph)) Γ σ A :
+  let ext := get_ctx_lift cat (of_global_context Σ) (last_condition σ) in
+  type_local_env Σ Γ ->
+  (of_global_context Σ) ## Γ |= σ ->
+  Σ ;;; Γ ,,, ext |- [A]ᵗ Σ (σ ,, fcLift) : (⟦ tSort [Universe.Expr.set] ⟧ᵀ) Σ (σ ,, fcLift) ->
+  Σ ;;; Γ |- ⟦A⟧! Σ σ :  tSort (Universe.sup [Universe.Expr.set] [Universe.Expr.set]).
+Proof.
+  simpl.
+  intros TyCtx FcValid H.
+  unfold ft_type_boxed,otranslate_boxed_type. simpl.
+  destruct (otranslate_type otranslate (of_global_context Σ)
+            (extend_forcing_ctx {| f_context := σ; f_category := cat; f_translator := [] |} fcLift)
+            tt A) eqn: HA.
+  simpl. eapply type_Prod.
+  - apply obj_sort.
+  - replace ([Universe.Expr.set]) with
+        (Universe.sup [Universe.Expr.set] [Universe.Expr.set]) by reflexivity.
+    eapply type_Prod.
+    pose ([vass pos_name Relevant (tConst "Obj" [])]) as Γ'.
+    eapply hom_sort.
+    + change (Σ;;; Γ ,,, Γ' |- lift0 #|Γ'| (tRel (last_condition σ)) : lift0 #|Γ'| (cat_obj)).
+      subst Σ. eapply weakening.
+      * apply typed_empty_global_env.
+      * simpl. constructor;eauto.
+        econstructor. apply obj_sort.
+      * apply last_condition_sound;eauto.
+    + solve_rel.
+    + unfold mkOptApp. apply type_translation_sound.
+      * apply  ctx_with_lift_sound;eauto.
+      * constructor. assumption.
+      * apply H.
+Qed.
+
+(* Lemma ctx_translation_extension (Σ := ([],init_graph)) σ Γ : *)
+(*   let E := of_global_context Σ in *)
+(*   ⟦ Γ ⟧ Σ (σ,, fcLift) = Γ ,,, (get_ctx_lift cat E (last_condition σ)). *)
+(* Proof. *)
+(*   simpl. destruct Γ. *)
+(*   - unfold ft_ctx,otranslate_context_no_sigma. simpl. cbv. *)
+
+Lemma forcing_typing_soundness (Σ := ([],init_graph)) Γ t T σ  :
   type_local_env Σ Γ ->
   Σ ;;; Γ |- t : T ->
   let Σ' := Σ in
   Σ' ;;; (⟦Γ⟧ Σ σ) |- ([t]ᵗ Σ σ) : (⟦T⟧ᵀ Σ σ).
 Proof.
   intros TyCtx Ty.
-  induction Ty; simpl.
+  revert σ.
+  induction Ty; intros; simpl.
   - (* -- Variables -- *)
     simpl. unfold translate_var.
     unshelve econstructor; simpl.
     Focus 2. constructor.  admit.
   - (* -- Sorts -- *)
+    assert (FcValid : of_global_context Σ ## (⟦ Γ ⟧) Σ σ |= σ) by
+        (apply context_traslation_valid;auto).
     (* Simplifying the applications in the type first*)
       unfold ft_term,otranslate,lambda_prefix,extend.
       eapply type_Conv;simpl.
-      * apply lam_q_f_sound;simpl;auto.
+      * apply lam_q_f_sound;simpl.
         ** apply forcing_context_soundness;assumption.
+        ** apply FcValid.
         ** eapply Π_q_f_lift_sound; apply type_Sort.
       * unfold ft_type. simpl in *. unfold mkOptApp.
         eapply type_App.
         ** eapply lam_q_f_sound;simpl.
            *** apply forcing_context_soundness;assumption.
+           *** apply FcValid.
            *** apply Π_q_f_lift_sound. unfold Universe.super. simpl.
                unfold Universe.type1,Universe.Expr.type1.
            (* TODO: show that [tSort [(Level.set, true)]] has type [tSort l] for some level l *)
@@ -235,13 +345,14 @@ Proof.
            type_spine_step. apply id_hom_type. solve_last_cond.
            apply type_spine_nil.
       * simpl. unfold ft_type. simpl. unfold mkOptApp.
+        (* Abstract this reduction to a tactic *)
         eapply cumul_red_r. Focus 2.
         eapply red_beta. simpl.
         eapply cumul_red_r. Focus 2.
         eapply red_beta. simpl.
         eapply cumul_refl.
         simpl.
-        (* NOTE: not sure how to prove this stuff about [leq_universe]  *)
+        (* NOTE: not sure how to prove this stuff about [leq_universe] *)
         assert (H : leq_universe
                       init_graph
                       (Universe.sup [Universe.Expr.set]
@@ -249,17 +360,52 @@ Proof.
                       (Universe.super l) = true). admit.
         rewrite H. rewrite Nat.eqb_refl. reflexivity.
   - admit.
-  - (* Products *)
+  - (* -- Products -- *)
+    assert (CtxSound : type_local_env Σ (⟦Γ⟧ Σ σ)) by (apply forcing_context_soundness;auto).
+    assert (FcValid : of_global_context Σ ## (⟦ Γ ⟧) Σ σ |= σ) by
+        (apply context_traslation_valid;auto).
+    rename t into A. rename b into B.
+    unfold ft_type, ft_term,snd. simpl.
+    destruct (otranslate_boxed_type otranslate (of_global_context Σ)
+            (extend_forcing_ctx {| f_context := σ; f_category := cat; f_translator := nil |} fcLift)
+            tt A) as [sigma t_] eqn:Ht.
+    destruct (otranslate_type otranslate (of_global_context Σ)
+            (add_variable
+               (extend_forcing_ctx {| f_context := σ; f_category := cat; f_translator := nil |}
+                                   fcLift)) sigma B) as [sigma0 u_] eqn:Hu.
+    unfold mkOptApp.
+    eapply type_Conv;simpl.
+    * eapply lam_q_f_sound;simpl.
+      ** apply forcing_context_soundness;assumption.
+      ** apply FcValid.
+      ** eapply type_Prod.
+         *** eapply Π_q_f_lift_sound.
+             eapply type_translation_sound.
+             **** simpl.
+                  pose [vass hom_name Relevant (tApp cat_hom [tRel 2; tRel 0]);
+                        vass pos_name Relevant cat_obj] as Γ'.
+                  pose [vass hom_name Relevant (tApp cat_hom [tRel (S (last_condition σ)); tRel 0]);
+                        vass pos_name Relevant (tConst "Obj" [])] as Γ''.
+                  change (type_local_env ([], init_graph) (⟦ Γ ⟧ Σ σ ,,, Γ'' ,,, Γ')).
+                  eapply ctx_with_lift_sound with (σ := σ ,, fcLift);eauto.
+                  eapply ctx_with_lift_sound with (σ := σ);eauto.
+                  constructor;eauto.
+             **** repeat constructor;eauto.
+             **** simpl.
+                  pose [vass hom_name Relevant (tApp cat_hom [tRel 2; tRel 0]);
+                        vass pos_name Relevant cat_obj] as Γ'.
+                  pose [vass hom_name Relevant (tApp cat_hom [tRel (S (last_condition σ)); tRel 0]);
+                        vass pos_name Relevant (tConst "Obj" [])] as Γ''.
+                  assert (Hs1 :[Universe.Expr.set] = s1). admit.
+                  rewrite Hs1. simpl in IHTy1.
+                  change
+  (Σ ;;; (⟦ Γ ⟧) Σ σ ,,, Γ'' ,,, Γ' |- [A ]ᵗ Σ (σ,, fcLift,, fcLift) : (⟦ tSort s1 ⟧ᵀ Σ  (σ,, fcLift,, fcLift))).
+                  pose ((⟦ Γ ⟧) Σ ((σ,, fcLift),, fcLift)) as G.
+                  unfold ft_ctx in G.
+                  (* assert (Hfc : of_global_context Σ ## G |= (σ ,, fcLift ,, fcLift)). *)
+                  (* { constructor. } *)
+                  (* simpl in G. *)
+                  (* eapply IHTy1 with (σ := σ ,,fcLift,,fcLift). *)
+                  admit.
 
-       (* econstructor;simpl. Focus 4. *)
-       (* eapply cumul_red_r. *)
-       (* Focus 2. eapply red_beta. simpl. *)
-       (* eapply cumul_red_r. *)
-       (* Focus 2. eapply red_beta. simpl. *)
-       (* eapply cumul_refl. apply leq_refl. *)
-       (* econstructor. *)
-       (* apply obj_sort. *)
-       (* econstructor. econstructor.  *)
-
-               (* econstructor. econstructor. *)
 Admitted.
